thys/LLL_Basis_Reduction/LLL_Complexity.thy
@@ -16,153 +16,184 @@ theory LLL_Complexity
   imports LLL 
 begin
 
-context
-  fixes body_cost :: nat
-begin
+type_synonym 'a cost = "'a \<times> nat" 
 
-context
-  fixes \<alpha> :: rat and m :: nat 
-begin
+definition cost :: "'a cost \<Rightarrow> nat" where "cost = snd" 
+definition result :: "'a cost \<Rightarrow> 'a" where "result = fst" 
 
-definition basis_reduction_step_cost :: "state \<Rightarrow> state \<times> nat" where
-  "basis_reduction_step_cost state = (basis_reduction_step \<alpha> state, body_cost)"
-
-partial_function (tailrec) basis_reduction_main_cost :: "state \<times> nat \<Rightarrow> state \<times> nat" where
-  [code]: "basis_reduction_main_cost state_cost = (case state_cost of (state, cost) \<Rightarrow>
-     case state of (i,F,G) \<Rightarrow>
-     if i < m
-     then case basis_reduction_step_cost state of 
-       (state',c) \<Rightarrow> basis_reduction_main_cost (state', c + cost) 
-     else state_cost)"
-end
-
-definition basis_reduction_state_cost :: "nat \<Rightarrow> rat \<Rightarrow> int vec list \<Rightarrow> state \<times> nat" where 
-  "basis_reduction_state_cost n \<alpha> F = basis_reduction_main_cost \<alpha> (length F) (initial_state n F, 0)" 
-
-
-definition reduce_basis_cost :: "nat \<Rightarrow> rat \<Rightarrow> int vec list \<Rightarrow> int vec list \<times> nat" where
-  "reduce_basis_cost n \<alpha> F = (\<lambda> (state, cost). ((of_list_repr o fst o snd) state, cost))
-     (basis_reduction_state_cost n \<alpha> F)" 
-end
+lemma cost_simps: "cost (a,c) = c" "result (a,c) = a" 
+  unfolding cost_def result_def by auto
 
 context LLL
 begin
 
-context fixes \<alpha> :: rat and body_cost :: nat
- assumes \<alpha>: "\<alpha> > 4/3"
+context
+  fixes \<alpha> :: rat and L :: "int vec set"
+  assumes \<alpha>: "\<alpha> > 4/3" and m0: "m \<noteq> 0" 
 begin
 
 private lemma alpha: "\<alpha> \<ge> 4/3" using \<alpha> by auto
 
-context fixes L :: "int vec set" and A :: nat
+context
+  fixes body_cost initial_gso_cost :: nat
 begin
 
-lemma basis_reduction_main_cost: fixes F G assumes "LLL_invariant L \<alpha> A state F G"
-  and "basis_reduction_main_cost body_cost \<alpha> m (state,c) = (state',c')" 
-shows "basis_reduction_main \<alpha> m state = state' \<and> c' \<le> c + body_cost * LLL_measure \<alpha> state"
-  using assms
-proof (induct state arbitrary: F G c rule: wf_induct[OF wf_measure[of "LLL_measure \<alpha>"]])
-  case (1 state F G c)
-  note inv = 1(2)
-  note IH = 1(1)[rule_format]
-  note res = 1(3)
-  obtain i Fr1 Gr1 where state: "state = (i,Fr1,Gr1)" by (cases state, auto)
-  note inv = inv[unfolded state]
-  show ?case
-  proof (cases "i < m")
-    case True
-    with inv have i: "i < m" unfolding LLL_invariant_def by auto
-    obtain state'' where b: "basis_reduction_step \<alpha> (i, Fr1, Gr1) = state''" by auto
-    from res[unfolded basis_reduction_main_cost.simps[of _ _ _ "(state,c)"], unfolded state b split
-        basis_reduction_step_cost_def] True
-    have res: "basis_reduction_main_cost body_cost \<alpha> m (state'', body_cost + c) = (state', c')" by auto 
-    note bsr = basis_reduction_step[OF alpha inv i b]
-    from bsr(1) obtain F' G' where inv: "LLL_invariant L \<alpha> A state'' F' G'" by auto
-    from bsr(2) have "(state'' ,state) \<in> measure (LLL_measure \<alpha>)" by (auto simp: state)
-    from IH[OF this inv res] have
-      res': "basis_reduction_main \<alpha> m state'' = state'" 
-      and c: "c' \<le> c + body_cost * (Suc (LLL_measure \<alpha> state''))" by auto
-    have res: "basis_reduction_main \<alpha> m state = state'"
-      unfolding basis_reduction_main.simps[of _ _ state] unfolding state split b res' using True by auto
-    show ?thesis
-      by (intro conjI res, rule order.trans[OF c add_left_mono[OF mult_left_mono]],
-        insert bsr(2) state, auto)
-  next
-    case False
-    from False res have state': "state' = (i, Fr1, Gr1)" and c: "c' = c"
-      and res: "basis_reduction_main \<alpha> m state = (i, Fr1, Gr1)" 
-      unfolding basis_reduction_main_cost.simps[of _ _ _ "(state,c)"] 
-        basis_reduction_main.simps[of _ _ state] unfolding split state by auto
-    from False LLL_invD[OF inv] have im: "i = m" by auto
-    show ?thesis unfolding state' fst_conv c
-      by (intro conjI im res, auto)
-  qed
+definition basis_reduction_step_cost :: "state \<Rightarrow> state cost" where
+  "basis_reduction_step_cost state = (basis_reduction_step \<alpha> state, body_cost)"
+
+lemma basis_reduction_step_cost: "cost (basis_reduction_step_cost state) \<le> body_cost" 
+  "result (basis_reduction_step_cost state) = basis_reduction_step \<alpha> state" 
+  unfolding basis_reduction_step_cost_def cost_simps by auto
+
+function basis_reduction_main_cost :: "state \<Rightarrow> state cost" where
+  "basis_reduction_main_cost state = (
+     case state of (i,F,G) \<Rightarrow>
+     if i < m \<and> (\<exists> A FF GG. LLL_invariant L \<alpha> A state FF GG) 
+       \<comment> \<open>The check on the invariant is just to be able to prove termination. 
+          One cannot use partial-function at this point, since the function with cost is not tail-recursive.\<close>
+     then case basis_reduction_step_cost state of 
+       (state1,c1) \<Rightarrow> 
+       case basis_reduction_main_cost state1 of
+       (state2,c2) \<Rightarrow> (state2, c1 + c2)
+     else (state, 0))"
+  by pat_completeness auto
+
+termination
+proof (standard, rule wf_measure[of "LLL_measure \<alpha>"], goal_cases)
+  case (1 state i FG F G state1 c1)
+  note * = 1(1)[symmetric] 1(2)[symmetric] 1(3) 1(4)[symmetric]
+  from * obtain FF GG A where i: "i < m" and inv: "LLL_invariant L \<alpha> A (i, F, G) FF GG" by auto
+  from basis_reduction_step_cost[of state, unfolded *(4)] 
+  have res: "basis_reduction_step \<alpha> (i, F, G) = state1" unfolding * cost_simps by auto
+  from basis_reduction_step[OF alpha inv i res]
+  show ?case unfolding * by auto
 qed
-end
+
+declare basis_reduction_main_cost.simps[simp del]
+
+definition "num_loops A = nat (ceiling (m + 2 * m * m * log (4 * of_rat \<alpha> / (4 + of_rat \<alpha>)) (real A)))"
+
+lemma basis_reduction_main_cost: fixes F G assumes "LLL_invariant L \<alpha> A state F G"
+  shows "result (basis_reduction_main_cost state) = basis_reduction_main \<alpha> m state" (is ?g1) 
+   "cost (basis_reduction_main_cost state) \<le> body_cost * num_loops A" (is ?g2)
+proof -
+  have ?g1 and cost: "cost (basis_reduction_main_cost state) \<le> body_cost * LLL_measure \<alpha> state"
+    using assms
+  proof (atomize (full), induct state arbitrary: F G rule: wf_induct[OF wf_measure[of "LLL_measure \<alpha>"]])
+    case (1 state F G)
+    note inv = 1(2)
+    have ex: "(\<exists>A FF. Ex (LLL_invariant L \<alpha> A state FF)) = True" using inv by auto
+    note IH = 1(1)[rule_format]
+    obtain i Fr1 Gr1 where state: "state = (i,Fr1,Gr1)" by (cases state, auto)
+    note inv = inv[unfolded state]
+    note simp = basis_reduction_main_cost.simps[of state, unfolded state split, folded state, unfolded ex]
+    show ?case
+    proof (cases "i < m")
+      case i: True
+      obtain c1 state1 where b: "basis_reduction_step_cost (i, Fr1, Gr1) = (state1, c1)" (is "?b = _")
+        by (cases ?b, auto)
+      note simp = simp[unfolded state b split, folded state]
+      from basis_reduction_step_cost[of state, unfolded state b cost_simps]
+      have c1: "c1 \<le> body_cost" and bb: "basis_reduction_step \<alpha> (i, Fr1, Gr1) = state1" by auto
+      obtain c2 state2 where rec: "basis_reduction_main_cost state1 = (state2, c2)" (is "?rec = _")
+        by (cases ?rec, auto)
+      note simp = simp[unfolded rec split]
+      from simp i have res: "basis_reduction_main_cost state = (state2, c1 + c2)" by auto    
+      note bsr = basis_reduction_step[OF alpha inv i bb]
+      from bsr(1) obtain F' G' where inv: "LLL_invariant L \<alpha> A state1 F' G'" by auto
+      from bsr(2) have "(state1 ,state) \<in> measure (LLL_measure \<alpha>)" by (auto simp: state)
+      from IH[OF this inv, unfolded rec cost_simps]
+      have res': "basis_reduction_main \<alpha> m state1 = state2" 
+        and c2: "c2 \<le> body_cost * LLL_measure \<alpha> state1" by auto
+      have res': "basis_reduction_main \<alpha> m state = state2"
+        unfolding basis_reduction_main.simps[of _ _ state] unfolding split b state bb res' using i by auto
+      from bsr(2)[folded state] obtain k where meas: "LLL_measure \<alpha> state = Suc (LLL_measure \<alpha> state1) + k" 
+        and "k = LLL_measure \<alpha> state - Suc (LLL_measure \<alpha> state1)" by simp 
+      show ?thesis unfolding res' res cost_simps
+        by (intro conjI[OF refl], rule order.trans[OF add_mono[OF c1 c2]], unfold meas, auto)
+    next
+      case False
+      thus ?thesis unfolding simp basis_reduction_main.simps[of _ _ state] unfolding state split
+        by (auto simp: cost_simps)
+    qed
+  qed
+  show ?g1 by fact
+  obtain i F G where state: "state = (i, F, G)" by (cases state, auto)
+  note cost also have "body_cost * LLL_measure \<alpha> state \<le> body_cost * num_loops A" 
+    by (rule mult_left_mono, unfold num_loops_def, insert 
+    LLL_measure_approx[OF alpha assms[unfolded state] \<alpha> m0, folded state], linarith+)
+  finally show ?g2 . 
+qed
+
+definition initial_state_cost :: "int vec list \<Rightarrow> state cost" where
+  "initial_state_cost F = (let G = gram_schmidt_triv n (map (map_vec of_int) F);
+     Fr = ([], F);
+     Gr = ([], G)
+     in ((0, Fr, Gr), initial_gso_cost))" 
+
+lemma initial_state_cost: "cost (initial_state_cost F) \<le> initial_gso_cost" 
+  "result (initial_state_cost F) = initial_state n F" 
+  unfolding initial_state_cost_def initial_state_def Let_def cost_simps by auto
+
+definition basis_reduction_state_cost :: "int vec list \<Rightarrow> state cost" where 
+  "basis_reduction_state_cost F = (case initial_state_cost F of
+     (state1,c1) \<Rightarrow> case basis_reduction_main_cost state1
+     of (state2,c2) \<Rightarrow> (state2,c1 + c2))" 
+
+definition reduce_basis_cost :: "int vec list \<Rightarrow> int vec list cost" where
+  "reduce_basis_cost F = (case basis_reduction_state_cost F of (state,c) \<Rightarrow> 
+    ((of_list_repr o fst o snd) state, c))" 
+
+definition "A (F :: int vec list) = max_list (map (nat o sq_norm) F)" 
 
 context
   fixes F :: "int vec list" 
   assumes len: "length F = m"
-    and lin_dep: "gs.lin_indpt_list (RAT F)" 
-    and m0: "m \<noteq> 0" 
+  and lin_dep: "gs.lin_indpt_list (RAT F)" 
+  and L: "lattice_of F = L" 
 begin
 
-qualified definition "A = max_list (map (nat o sq_norm) F)" 
-qualified definition "num_loops = m + 2 * m * m * log (4 * of_rat \<alpha> / (4 + of_rat \<alpha>)) A"
-
-lemma basis_reduction_state_cost: assumes res: "basis_reduction_state_cost body_cost n \<alpha> F = (state,c)"
-shows "basis_reduction_state n \<alpha> F = state" 
-  "c \<le> body_cost * num_loops" 
+lemma basis_reduction_state_cost: 
+   "result (basis_reduction_state_cost F) = basis_reduction_state n \<alpha> F"  (is ?g1)
+   "cost (basis_reduction_state_cost F) \<le> initial_gso_cost + body_cost * num_loops (A F)" (is ?g2)
 proof -
-  let ?init = "initial_state n F" 
-  from res[unfolded basis_reduction_state_cost_def len]
-  have res_main: "basis_reduction_main_cost body_cost \<alpha> m (?init, 0) = (state, c)" by auto
-  from initial_state[OF alpha lin_dep len refl A_def]
-  obtain F' G' where inv: "LLL_invariant (lattice_of F) \<alpha> A ?init F' G'" by auto
-  from basis_reduction_main_cost[OF this res_main]
-  have "basis_reduction_main \<alpha> m ?init = state" 
-    and c: "c \<le> body_cost * LLL_measure \<alpha> ?init" by auto
-  thus "basis_reduction_state n \<alpha> F = state" unfolding basis_reduction_state_def len by auto
-  obtain i Fr Gr where init: "?init = (i,Fr,Gr)" by (cases ?init, auto)
-  from LLL_measure_approx[OF alpha inv[unfolded init] \<alpha> m0, folded init]
-  have num: "real (LLL_measure \<alpha> (initial_state n F)) \<le> num_loops" unfolding num_loops_def .
-  have "real c \<le> body_cost * (real (LLL_measure \<alpha> ?init))" using c
-    using SN_Orders.of_nat_mono by force
-  also have "\<dots> \<le> body_cost * num_loops" 
-    by (rule mult_left_mono[OF num], auto)
-  finally show "c \<le> body_cost * num_loops" .
+  obtain state1 c1 where init: "initial_state_cost F = (state1, c1)" (is "?init = _") by (cases ?init, auto)
+  obtain state2 c2 where main: "basis_reduction_main_cost state1 = (state2, c2)" (is "?main = _") by (cases ?main, auto)
+  have res: "basis_reduction_state_cost F = (state2, c1 + c2)" 
+    unfolding basis_reduction_state_cost_def init main split by simp
+  from initial_state_cost[of F, unfolded init cost_simps]
+  have c1: "c1 \<le> initial_gso_cost" and init: "initial_state n F = state1" by auto
+  from initial_state[OF alpha lin_dep len init refl, folded A_def] L
+  obtain F' G' where inv: "LLL_invariant L \<alpha> (A F) state1 F' G'" by auto
+  from basis_reduction_main_cost[OF inv, unfolded main cost_simps]
+  have main: "basis_reduction_main \<alpha> m state1 = state2" and c2: "c2 \<le> body_cost * num_loops (A F)" 
+    by auto
+  have res': "basis_reduction_state n \<alpha> F = state2" unfolding basis_reduction_state_def len init main ..
+  show ?g1 unfolding res res' cost_simps ..
+  show ?g2 unfolding res cost_simps using c1 c2 by auto
 qed
 
-text \<open>The lemma for the LLL algorithm with explicit cost @{const reduce_basis_cost}
+text \<open>The lemma for the LLL algorithm with explicit cost annotations @{const reduce_basis_cost}
   shows that the termination measure
-  is indeed a bound for the explicit costs. Moreover, we get the same result
-  as in the non-cost counting @{const reduce_basis}. Therefore, we can easily
-  carry over results derived for @{const reduce_basis}.\<close>
+  indeed gives rise to an explicit cost bound. Moreover, the computed result is
+  the same as in the non-cost counting @{const reduce_basis}.\<close>
 
-lemma reduce_basis_cost: assumes res: "reduce_basis_cost body_cost n \<alpha> F = (F',c)" 
-  shows "c \<le> body_cost * num_loops" (is ?g1)
-    "reduce_basis n \<alpha> F = (F', gram_schmidt n (RAT F'))" (is ?g2)
-    "lattice_of F = lattice_of F'" (is ?g3)
-    "gs.reduced \<alpha> m (gram_schmidt n (RAT F')) (gs.\<mu> (RAT F'))" (is ?g4)
+lemma reduce_basis_cost: 
+   "result (reduce_basis_cost F) = fst (reduce_basis n \<alpha> F)"  (is ?g1)
+   "cost (reduce_basis_cost F) \<le> initial_gso_cost + body_cost * num_loops (A F)" (is ?g2)
 proof -
-  let ?basis = "basis_reduction_state_cost body_cost n \<alpha> F" 
-  from res[unfolded reduce_basis_cost_def]
-  obtain state where res': "?basis = (state, c)" 
-    and F': "F' = (of_list_repr \<circ> fst \<circ> snd) state" by (cases ?basis, auto)
-  from basis_reduction_state_cost[OF res']
-  have res': "basis_reduction_state n \<alpha> F = state" 
-    and c: "c \<le> body_cost * num_loops" by auto 
-  obtain G' where res: "reduce_basis n \<alpha> F = (F', G')" unfolding F' reduce_basis_def res' by auto
-  show ?g1 by fact
-  note reduce = reduce_basis[OF alpha lin_dep len res]
-  show ?g2 unfolding res using reduce by auto
-  show ?g3 by fact
-  show ?g4 using reduce by auto
+  obtain state c where b: "basis_reduction_state_cost F = (state,c)" (is "?b = _") by (cases ?b, auto)
+  from basis_reduction_state_cost[unfolded b cost_simps]
+  have bb: "basis_reduction_state n \<alpha> F = state" and c: "c \<le> initial_gso_cost + body_cost * num_loops (A F)" 
+    by auto
+  show ?g1 ?g2 unfolding reduce_basis_cost_def reduce_basis_def b bb split cost_simps fst_conv using c by auto
 qed
 
-thm reduce_basis_cost(1)[unfolded A_def num_loops_def]
+text \<open>Theorem with expanded costs\<close>
+thm reduce_basis_cost(2)[unfolded num_loops_def A_def]
 
-end (* common assumption on fs, like lin-indep *)
+end (* lin-indep F *)
+end (* fixing body_cost and initial_gso_cost *)
 end (* fixing \<alpha> and assume \<alpha> > 4/3 *)
 end (* LLL locale which just fixes n and m *)
 end (* theory *)
